More parser lemmas

src/chess/algebraic.lean
@@ -5,7 +5,7 @@ open chess
 
 namespace chess
 
-open piece
+open piece parser list (mfirst)
 
 namespace piece
 
@@ -33,21 +33,85 @@ def piece_repr : piece → string
 | ♘ := "♘"
 | ♙ := "♙"
 
+abbreviation promotions : Type := {p : piece // p = ♕ ∨ p = ♖ ∨ p = ♗ ∨ p = ♘}
+
 instance : has_repr piece := ⟨piece_repr⟩
 
-def parser (x : piece) : parser piece :=
-(parser.ch x.char_symbol <|> parser.ch x.unicode_symbol) $> x
+def parser' (x : piece) : parser piece :=
+(ch x.char_symbol <|> ch x.unicode_symbol) $> x
+
+def promotions.parser' : parser piece :=
+decorate_error "<promotions>" $ mfirst parser' [queen, rook, bishop, knight]
+
+-- lemma promotions.parser'_not_king (cb n) (h : promtions.parser' cb n ≠ parse_result.fail): promotions.parser' cb n
+
+def parser : parser piece :=
+decorate_error "<piece>" $ mfirst parser' [king, queen, rook, bishop, knight, pawn]
 
 end piece
 
-def parser : parser piece :=
-asum (piece.parser <$> [king, queen, rook, bishop, knight, pawn])
+@[derive [decidable_eq, fintype]]
+inductive capture
+| capture
+| noncapture
 
-#eval parser.run_string (chess.parser) "♗"
-#eval parser.run_string (chess.parser) "K"
-#eval parser.run_string (chess.parser) "N"
-#eval parser.run_string (chess.parser.many) "KQRBNP"
-#eval parser.run_string (chess.parser.many) "KQRBNX"
+def capture.repr : capture → string
+| capture.capture := "capture"
+| capture.noncapture := "noncapture"
 
+instance capture_has_repr : has_repr capture := ⟨capture.repr⟩
+
+variables {α β : Type} [has_zero α] [has_one α] [has_add α] [has_zero β] [has_one β] [has_add β]
+
+def file.parser' : parser α := numeral.char 'a' 'z' _
+def file.parser [fintype α] : parser α := numeral.char.of_fintype 'a' _
+def rank.parser' : parser α := numeral.from_one α
+def rank.parser [fintype α] : parser α := numeral.from_one.of_fintype α
+def square.parser' : parser (α × β) :=
+(λ x y, ⟨y, x⟩) <$> file.parser' <*> rank.parser'
+def square.parser [fintype α] [fintype β] : parser (α × β) :=
+(λ x y, ⟨y, x⟩) <$> file.parser <*> rank.parser
+def square.parser.optional [fintype α] [fintype β] : parser (option α × option β) :=
+(λ x y, ⟨y, x⟩) <$> (some <$> file.parser <|> pure none) <*> (some <$> rank.parser <|> pure none)
+def capture.parser : parser capture :=
+ch 'x' $> capture.capture <|> pure capture.noncapture
+
+variables (α β)
+
+structure move.description :=
+(figure : piece)
+(from_sq : (option α × option β))
+(to_sq : (α × β))
+(capture : capture)
+
+instance move.description.has_repr [has_repr α] [has_repr β] : has_repr (move.description α β) :=
+⟨λ ⟨p, fsq, tsq, c⟩, string.intercalate " " [repr p, repr fsq, repr tsq, repr c]⟩
+
+structure pawn.capture.description extends move.description α β :=
+(promoted : {p : piece // p ≠ pawn ∧ p ≠ king})
+
+variables {α β}
+
+def move.parser [fintype α] [fintype β] : parser (move.description α β) :=
+(λ p fsq c tsq, ⟨p, fsq, tsq, c⟩) <$> piece.parser <*> square.parser.optional <*> capture.parser <*> square.parser
+
+#eval run_string (piece.parser) "♗"
+#eval run_string (piece.parser) "K"
+#eval run_string (piece.parser) "N"
+#eval run_string (piece.parser) "x"
+#eval run_string (piece.parser.many) "KQRBNP"
+#eval run_string (piece.parser.many) "KQRBNX"
+
+#eval run_string (numeral (fin 300)) "001334"
+#eval run_string (@file.parser' (fin 300) _ _ _) "a"
+#eval run_string (@file.parser (fin 8) _ _ _ _) "a"
+#eval run_string (@file.parser (fin 8) _ _ _ _) "h"
+#eval run_string (@file.parser (fin 8) _ _ _ _) "i"
+#eval run_string (@rank.parser (fin 300) _ _ _ _) "4"
+#eval run_string (@square.parser (fin 300) (fin 300) _ _ _ _ _ _ _ _) "a4"
+
+#eval run_string capture.parser ""
+
+#eval run_string (@move.parser (fin 8) (fin 8) _ _ _ _ _ _ _ _) "Qd5xc8"
 
 end chess
