src/chess/algebraic/utils.lean
@@ -1,7 +1,531 @@
-import data.sum
+import data.nat.cast
+import data.fintype.card
+import utils.list
 
 instance has_repr_sum {α β : Type*} [has_repr α] [has_repr β] : has_repr (α ⊕ β) :=
 ⟨sum.elim (λ x, "sum.inl " ++ repr x) (λ x, "sum.inr " ++ repr x)⟩
 
-def asum {α : Type*} {m : Type* → Type*} [alternative m] (xs : list (m α)) : m α :=
-xs.foldl (<|>) failure
+@[simp] lemma dlist_singleton {α : Type*} {a : α} : dlist.singleton a = dlist.lazy_of_list ([a]) := rfl
+
+open parser parse_result
+
+@[simp] def parse_result.pos {α} : parse_result α → ℕ
+| (done n _) := n
+| (fail n _) := n
+
+namespace parser
+
+section numeral
+
+def numeral (α : Type) [has_zero α] [has_one α] [has_add α] : parser α :=
+nat.cast <$> nat
+
+def numeral.of_fintype (α : Type) [has_zero α] [has_one α] [has_add α] [fintype α] : parser α :=
+do
+  c ← nat,
+  guard (c < fintype.card α),
+  pure c
+
+def numeral.from_one (α : Type) [has_zero α] [has_one α] [has_add α] : parser α :=
+do
+  c ← nat,
+  guard (0 < c),
+  pure $ ((c - 1) : ℕ)
+
+def numeral.from_one.of_fintype (α : Type) [has_zero α] [has_one α] [has_add α] [fintype α] : parser α :=
+do
+  c ← nat,
+  guard (0 < c),
+  guard (c ≤ fintype.card α),
+  pure $ ((c - 1) : ℕ)
+
+def numeral.char (fromc toc : char) (α : Type) [has_zero α] [has_one α] [has_add α] : parser α :=
+do
+  c ← sat (λ c, fromc ≤ c ∧ c ≤ toc),
+  pure $ ((c.to_nat - fromc.to_nat) : ℕ)
+
+def numeral.char.of_fintype (fromc : char) (α : Type) [has_zero α] [has_one α] [has_add α]
+  [fintype α] : parser α :=
+do
+  c ← sat (λ c, fromc ≤ c ∧ c.to_nat - fintype.card α < fromc.to_nat),
+  pure $ ((c.to_nat - fromc.to_nat) : ℕ)
+
+end numeral
+
+section defn_lemmas
+
+variables {α β : Type} (msgs : thunk (list string)) (msg : thunk string)
+variables (p q : parser α) (cb : char_buffer) (n n' : ℕ) {err : dlist string}
+variables {a : α} {b : β}
+
+@[simp] def failed : Prop :=
+  ∃ (n' : ℕ) (err : dlist string), p cb n = fail n' err
+
+def valid : Prop :=
+  ∀ (cb : char_buffer) (n : ℕ), n ≤ (p cb n).pos ∧ ((p cb n).pos ≤ cb.size → n ≤ cb.size)
+
+lemma fail_iff :
+  (∀ pos' result, p cb n ≠ done pos' result) ↔ ∃ (pos' : ℕ) (err : dlist string), p cb n = fail pos' err :=
+begin
+  cases p cb n,
+  { simp [exists_prop, not_not, exists_false, exists_eq_right',
+               iff_false, exists_eq', not_forall] },
+  { simp only [forall_const, ne.def, not_false_iff, exists_eq_right',
+               exists_eq', forall_true_iff] }
+end
+
+lemma fail_iff' :
+  (∀ pos' result, p cb n ≠ done pos' result) ↔ p.failed cb n :=
+by { rw failed, exact fail_iff _ _ _ }
+
+lemma success_iff :
+  (∀ pos' err, p cb n ≠ fail pos' err) ↔ ∃ (pos' : ℕ) (result : α), p cb n = done pos' result :=
+begin
+  cases p cb n,
+  { simp only [exists_eq_right', exists_eq', forall_const, ne.def, not_false_iff, forall_true_iff] },
+  { simp only [exists_eq_right', exists_eq', exists_prop, not_not, exists_false, iff_false,
+               not_forall] }
+end
+
+lemma success_iff' :
+  (¬ p.failed cb n) ↔ ∃ (pos' : ℕ) (result : α), p cb n = done pos' result :=
+by simp only [failed, not_exists, success_iff]
+
+variables {p q cb n n' msgs msg}
+
+lemma decorate_errors_fail (h : p cb n = fail n' err) :
+  @decorate_errors α msgs p cb n = fail n ((dlist.lazy_of_list (msgs ()))) :=
+begin
+  dunfold decorate_errors,
+  rw h,
+  refl
+end
+
+lemma decorate_errors_success (h : p cb n = done n' a) :
+  @decorate_errors α msgs p cb n = done n' a :=
+begin
+  dunfold decorate_errors,
+  rw h,
+  refl
+end
+
+lemma decorate_error_fail (h : p cb n = fail n' err) :
+  @decorate_error α msg p cb n = fail n ((dlist.lazy_of_list ([msg ()]))) :=
+decorate_errors_fail h
+
+lemma decorate_error_success (h : p cb n = done n' a) :
+  @decorate_error α msg p cb n = done n' a :=
+decorate_errors_success h
+
+@[simp] lemma decorate_errors_success_iff :
+  @decorate_errors α msgs p cb n = done n' a ↔ p cb n = done n' a :=
+begin
+  dunfold decorate_errors,
+  cases p cb n,
+  { rw decorate_errors },
+  { rw decorate_errors,
+    simp only }
+end
+
+@[simp] lemma decorate_error_success_iff :
+  @decorate_error α msg p cb n = done n' a ↔ p cb n = done n' a :=
+decorate_errors_success_iff
+
+@[simp] lemma decorate_errors_failure_iff :
+  @decorate_errors α msgs p cb n = fail n err ↔
+    err = dlist.lazy_of_list (msgs ()) ∧ ∃ np err', p cb n = fail np err' :=
+begin
+  dunfold decorate_errors,
+  cases p cb n,
+  { rw decorate_errors,
+    simp only [exists_false, and_false] },
+  { rw decorate_errors,
+    simp only [true_and, and_true, eq_self_iff_true, exists_eq_right', exists_eq', eq_comm] }
+end
+
+@[simp] lemma decorate_error_failure_iff :
+  @decorate_error α msg p cb n = fail n err ↔
+    err = dlist.lazy_of_list ([msg ()]) ∧ ∃ np err', p cb n = fail np err' :=
+decorate_errors_failure_iff
+
+@[simp] lemma return_eq_pure : (@return parser _ _ a) = pure a := rfl
+
+@[simp] lemma pure_eq_done : (@pure parser _ _ a) = λ _ n, done n a := rfl
+
+
+section bind
+
+variable {f : α → parser β}
+
+@[simp] lemma bind_eq_bind : p.bind f = p >>= f := rfl
+
+@[simp] lemma bind_eq_done :
+  (p >>= f) cb n = done n' b ↔
+  ∃ (np : ℕ) (a : α), p cb n = done np a ∧ f a cb np = done n' b :=
+begin
+  split,
+  { intro h,
+    simp_rw [←bind_eq_bind, parser.bind] at h,
+    cases p cb n with pos r pos err,
+    { refine ⟨pos, r, rfl, _⟩,
+      rw ←h,
+      refl },
+    { simpa only using h } },
+  { rintro ⟨r, pos, h⟩,
+    simp only [h, ←bind_eq_bind, parser.bind, eq_self_iff_true, and_self] }
+end
+
+@[simp] lemma bind_eq_fail :
+  (p >>= f) cb n = fail n' err ↔
+  (p cb n = fail n' err) ∨ (∃ (np : ℕ) (a : α), p cb n = done np a ∧ f a cb np = fail n' err)
+  :=
+begin
+  split,
+  { intro h,
+    simp_rw [←bind_eq_bind, parser.bind] at h,
+    cases p cb n with pos r pos err,
+    { rw ←h,
+      simp only [false_or, exists_false],
+      refine ⟨pos, r, by simp only [eq_self_iff_true, and_self], _⟩,
+      refl },
+    { simpa only [parser.bind, exists_false, or_false, false_and] using h } },
+  { rintro (h | ⟨r, n', h, h'⟩),
+    { simp only [←bind_eq_bind, parser.bind, h, eq_self_iff_true, and_self] },
+    { simp only [←h', ←bind_eq_bind, parser.bind, h] } }
+end
+
+@[simp] lemma and_then_eq_bind {α β : Type} {m : Type → Type} [monad m] (a : m α) (b : m β) :
+  a >> b = a >>= (λ _, b) := rfl
+
+lemma and_then_fail :
+  (p >> return ()) cb n = parse_result.fail n' err ↔ p cb n = fail n' err :=
+by simp only [and_then_eq_bind, return_eq_pure, exists_false, or_false, pure_eq_done,
+              bind_eq_fail, and_false]
+
+lemma and_then_success :
+  (p >> return ()) cb n = parse_result.done n' () ↔ ∃ a, p cb n = done n' a:=
+by simp only [pure_eq_done, and_then_eq_bind, and_true, bind_eq_done, exists_eq_right,
+              eq_iff_true_of_subsingleton, return_eq_pure, exists_and_distrib_right]
+
+lemma mmap_empty_eq_done {l : list α} {lb : list β} :
+  list.nil.mmap f cb n = done n' lb ↔ n = n' ∧ lb = [] :=
+by simp only [eq_comm, pure_eq_done, list.mmap_nil]
+
+lemma mmap_cons_eq_done {a : α} {l : list α} {b : β} {lb : list β} :
+  (a :: l).mmap f cb n = done n' (b :: lb) ↔
+  ∃ (na : ℕ), f a cb n = done na b ∧ l.mmap f cb na = done n' lb :=
+begin
+  simp only [list.mmap_cons, bind_eq_done, pure_eq_done],
+  split,
+  { rintro ⟨np, b', h, lb', np', h', rfl, rfl, rfl⟩,
+    exact ⟨np, h, h'⟩ },
+  { rintro ⟨np, h, h'⟩,
+    exact ⟨np, b, h, n', lb, h', rfl, rfl, rfl⟩ }
+end
+
+lemma mmap_imp_fail {l : list α} (h : l.mmap f cb n = fail n' err) :
+    ∃ (a ∈ l) (np : ℕ), f a cb np = fail n' err :=
+begin
+  induction l with hd tl hl generalizing n n',
+  { simpa only using h },
+  { simp only [list.mmap_cons, exists_false, or_false, pure_eq_done, bind_eq_fail, and_false] at h,
+    simp only [exists_prop, list.mem_cons_iff],
+    rcases h with h | ⟨b, nb, hb, h⟩,
+    { exact ⟨hd, or.inl rfl, n, h⟩, },
+    { obtain ⟨a, ha, h'⟩ := hl h,
+      exact ⟨a, or.inr ha, h'⟩ } }
+end
+
+lemma mmap'_empty_eq_done {l : list α} {lb : list β} :
+  list.nil.mmap' f cb n = done n' () ↔ n = n' :=
+by simp only [pure_eq_done, list.mmap'_nil, and_true, eq_iff_true_of_subsingleton]
+
+lemma mmap'_cons_eq_done {l : list α} :
+  (a :: l).mmap' f cb n = done n' () ↔
+  ∃ (na : ℕ) (b : β), f a cb n = done na b ∧ l.mmap' f cb na = done n' () :=
+by simp only [bind_eq_done, and_then_eq_bind, list.mmap'_cons]
+
+lemma mmap'_imp_fail {l : list α} (h : l.mmap' f cb n = fail n' err) :
+    ∃ (a ∈ l) (np : ℕ), f a cb np = fail n' err :=
+begin
+  induction l with hd tl hl generalizing n n',
+  { simpa only using h },
+  { simp only [bind_eq_fail, and_then_eq_bind, exists_and_distrib_right, list.mmap'_cons] at h,
+    simp only [exists_prop, list.mem_cons_iff],
+    rcases h with h | ⟨nb, -, h⟩,
+    { exact ⟨hd, or.inl rfl, n, h⟩, },
+    { obtain ⟨a, ha, h'⟩ := hl h,
+      exact ⟨a, or.inr ha, h'⟩ } }
+end
+
+end bind
+
+section map
+
+variable {f : α → β}
+
+@[simp] lemma map_eq_done : (f <$> p) cb n = done n' b ↔
+  ∃ (a : α), p cb n = done n' a ∧ f a = b :=
+begin
+  rw ←is_lawful_monad.bind_pure_comp_eq_map,
+  simp only [bind_eq_done, function.comp_app, pure_eq_done],
+  split,
+  { rintro ⟨np, a, h, rfl, rfl⟩,
+    exact ⟨a, h, rfl⟩ },
+  { rintro ⟨a, h, rfl⟩,
+    exact ⟨n', a, h, rfl, rfl⟩ }
+end
+
+@[simp] lemma map_eq_fail : (f <$> p) cb n = fail n' err ↔ p cb n = fail n' err :=
+by simp only [←bind_pure_comp_eq_map, exists_false, function.comp_app, or_false, pure_eq_done,
+              bind_eq_fail, and_false]
+
+end map
+
+@[simp] lemma orelse_eq_orelse : p.orelse q = (p <|> q) := rfl
+
+@[simp] lemma orelse_eq_done : (p <|> q) cb n = done n' a ↔
+  (p cb n = done n' a ∨ ((∃ err, p cb n = fail n err) ∧ q cb n = done n' a)) :=
+begin
+  rw ←orelse_eq_orelse,
+  split,
+  { intro h,
+    simp_rw parser.orelse at h,
+    cases p cb n with posp resp posp errp,
+    { left,
+      simpa only [parser.orelse] using h },
+    { right,
+      simp only [parser.orelse, ite_not] at h,
+      split_ifs at h with H H,
+      { cases q cb n with posq resq posq errq,
+        { simp only [parser.orelse] at h,
+          simp only [true_and, exists_eq', H, eq_self_iff_true, h] },
+        { simp only [parser.orelse] at h,
+          split_ifs at h;
+          exact h.elim } },
+      { exact h.elim } } },
+  { rintro (h | ⟨⟨err, h⟩, h'⟩),
+    { simp only [parser.orelse, h, eq_self_iff_true, and_self] },
+    { simp only [h, parser.orelse, eq_self_iff_true, not_true, if_false, ne.def],
+      cases q cb n with posq resq posq errq,
+      { simpa only [parser.orelse] using h' },
+      { simpa only using h' } } }
+end
+
+@[simp] lemma orelse_eq_fail_eq : (p <|> q) cb n = fail n err ↔
+  (p cb n = fail n err ∧ ∃ (nq errq), n < nq ∧ q cb n = fail nq errq) ∨
+  (∃ (errp errq), p cb n = fail n errp ∧ q cb n = fail n errq ∧ errp ++ errq = err)
+ :=
+begin
+  rw ←orelse_eq_orelse,
+  simp only [parser.orelse, exists_and_distrib_left],
+  cases p cb n with posp resp posp errp,
+  { simp only [parser.orelse, exists_false, false_and, or_self] },
+  by_cases h : posp = n,
+  { simp only [h, parser.orelse, true_and, eq_self_iff_true, not_true, if_false, ne.def,
+               exists_eq_left'],
+    cases q cb n with posq resq posq errq,
+    { simp only [parser.orelse, exists_false, and_false, false_and, or_self] },
+    { simp only [parser.orelse, exists_eq_right'],
+      split_ifs with H H',
+      { simp only [H, true_and, and_true, eq_self_iff_true, ne_of_gt H, exists_false, or_false,
+                   false_and] },
+      { have hn : posq ≠ n := ne_of_lt H',
+        have hl : posq ≤ n := le_of_not_lt H,
+        simp only [hn, hl, false_iff, not_and, not_lt, exists_false, or_false, false_and,
+                   forall_true_iff] },
+      { have : posq = n := le_antisymm (le_of_not_lt H) (le_of_not_lt H'),
+        simp only [this, lt_irrefl, true_and, false_or, eq_self_iff_true, exists_eq_left',
+                   and_false] } } },
+  { simp only [h, parser.orelse, if_true, exists_false, ne.def, not_false_iff, false_and, or_self] },
+end
+
+lemma orelse_eq_fail_invalid_lt (hn : n' < n) : (p <|> q) cb n = fail n' err ↔
+  (p cb n = fail n' err) ∨
+  (q cb n = fail n' err ∧ (∃ (errp), p cb n = fail n errp))
+ :=
+begin
+  rw ←orelse_eq_orelse,
+  simp only [parser.orelse, exists_and_distrib_left],
+  cases p cb n with posp resp posp errp,
+  { simp only [parser.orelse, exists_false, or_self, and_false] },
+  by_cases h : posp = n,
+  { simp only [h, parser.orelse, true_and, eq_self_iff_true, not_true, if_false, ne.def, and_true,
+               false_or, exists_eq', false_and, ne_of_gt hn],
+    cases q cb n with posq resq posq errq,
+    { simp only [parser.orelse, not_false_iff] },
+    { simp only [parser.orelse],
+      split_ifs with H H',
+      { have : posq ≠ n' := ne_of_gt (lt_trans hn H),
+        simp only [false_and, ne_of_gt hn, this] },
+      { simp only [iff_self] },
+      { have : posq = n := le_antisymm (le_of_not_lt H) (le_of_not_lt H'),
+        simp only [ne_of_gt hn, this, false_and] } } },
+  { simp only [h, parser.orelse, if_true, exists_false, ne.def, not_false_iff, false_and,
+               or_false, and_false] },
+end
+
+lemma orelse_eq_fail_of_valid_ne (hq : q.valid) (hn : n ≠ n') :
+  (p <|> q) cb n = fail n' err ↔ p cb n = fail n' err
+ :=
+begin
+  rw ←orelse_eq_orelse,
+  simp only [parser.orelse, exists_and_distrib_left],
+  cases p cb n with posp resp posp errp,
+  { simp [parser.orelse, exists_false, or_self, and_false] },
+  by_cases h : posp = n,
+  { simp only [h, parser.orelse, true_and, eq_self_iff_true, not_true, if_false, ne.def,
+               hn, and_true, false_or, exists_eq', false_and],
+    specialize hq cb n,
+    cases q cb n with posq resq posq errq,
+    { simp [parser.orelse] },
+    { simp only [parser.orelse, if_false],
+      simp only [parse_result.pos] at hq,
+      rcases eq_or_lt_of_le hq.left with rfl|H,
+      { simp only [lt_irrefl, hn, if_false, false_and] },
+      { simp only [H, if_true, hn, false_and] } } },
+  { simp only [h, parser.orelse, if_true, ne.def, not_false_iff] },
+end
+
+@[simp] lemma parser_eq_parser : @parser.failure α = failure := rfl
+
+@[simp] lemma failure_def : (failure : parser α) cb n = fail n dlist.empty := rfl
+
+lemma ch_of_empty (c : char) (cb : char_buffer) (h : cb.size = 0) (n : ℕ) :
+  ch c cb n = parse_result.fail n (dlist.singleton c.to_string) :=
+begin
+  rw ch,
+  rw sat,
+  rw eps,
+  simp only [pure_eq_done, and_then_eq_bind, decorate_error_failure_iff, true_and, dlist_singleton,
+             eq_self_iff_true],
+  use [n, dlist.empty],
+  simp only [h, not_lt, eq_self_iff_true, exists_false, zero_le, or_false, dif_neg, and_self,
+             bind_eq_fail, return_eq_pure, pure_eq_done]
+end
+
+section valid_parsers
+
+lemma pure.valid : valid (pure a) :=
+by { intros cb n, simp only [pure_eq_done, parse_result.pos, imp_self, and_true] }
+
+@[simp] lemma valid.bind {f : α → parser β} (hp : p.valid) (hf : ∀ a, (f a).valid) :
+  (p >>= f).valid :=
+begin
+  intros cb n,
+  specialize hp cb n,
+  cases hx : (p >>= f) cb n,
+  { obtain ⟨n', a, h, h'⟩ := bind_eq_done.mp hx,
+    specialize hf a cb n',
+    simp only [h', parse_result.pos] at hf,
+    simp only [h, parse_result.pos] at hp,
+    simp only [parse_result.pos],
+    split,
+    { exact le_trans hp.left hf.left },
+    { intro hn,
+      simp [hn, hf, hp] } },
+  { obtain h | ⟨n', a, h, h'⟩ := bind_eq_fail.mp hx,
+    { simpa only [h] using hp },
+    { specialize hf a cb n',
+      simp only [h', parse_result.pos] at hf,
+      simp only [h, parse_result.pos] at hp,
+      simp only [parse_result.pos],
+      split,
+      { exact le_trans hp.left hf.left },
+      { intro hn,
+        simp only [hn, hf, hp] } } },
+end
+
+lemma valid.and_then {q : parser β} (hp : p.valid) (hq : q.valid) :
+  (p >> q).valid :=
+by { rw [and_then_eq_bind], exact hp.bind (λ _, hq) }
+
+@[simp] lemma valid.map (hp : p.valid) {f : α → β} : (f <$> p).valid :=
+by { rw ←is_lawful_monad.bind_pure_comp_eq_map, exact hp.bind (λ _, pure.valid) }
+
+@[simp] lemma valid.mmap {l : list α} {f : α → parser β} (h : ∀ a ∈ l, (f a).valid) :
+  (l.mmap f).valid :=
+begin
+  induction l with hd tl hl generalizing h,
+  { exact pure.valid },
+  { exact valid.bind (h _ (list.mem_cons_self _ _))
+      (λ b, valid.map (hl (λ _ ha, h _ (list.mem_cons_of_mem _ ha)))) }
+end
+
+@[simp] lemma valid.mmap' {l : list α} {f : α → parser β} (h : ∀ a ∈ l, (f a).valid) :
+  (l.mmap' f).valid :=
+begin
+  induction l with hd tl hl generalizing h,
+  { exact pure.valid },
+  { refine valid.and_then (h _ (list.mem_cons_self _ _))
+      (hl (λ _ ha, h _ (list.mem_cons_of_mem _ ha))) }
+end
+
+@[simp] lemma failure.valid : @parser.valid α failure :=
+begin
+  simp only [failure_def, valid, imp_self, and_true, parse_result.pos],
+  rintro - _,
+  refl
+end
+
+@[simp] lemma valid.orelse (hp : p.valid) (hq : q.valid) : (p <|> q).valid :=
+begin
+  intros cb n,
+  cases hx : (p <|> q) cb n with posx resx posx errx,
+  { obtain h | ⟨⟨err, h⟩, h'⟩ := orelse_eq_done.mp hx,
+    { simpa only [h] using hp cb n },
+    { simpa only [h'] using hq cb n } },
+  { by_cases h : n = posx,
+    { simp only [hx, h, imp_self, and_true, parse_result.pos] },
+    { rw orelse_eq_fail_of_valid_ne hq h at hx,
+      simpa only [parse_result.pos, hx] using hp cb n } }
+end
+
+@[simp] lemma decorate_errors.valid (hp : p.valid) :
+  (@decorate_errors α msgs p).valid :=
+begin
+  dunfold decorate_errors,
+  intros cb n,
+  specialize hp cb n,
+  dsimp only,
+  cases p cb n,
+  { simpa only using hp },
+  { simp only [decorate_errors, imp_self, and_true, parse_result.pos] },
+end
+
+@[simp] lemma decorate_error.valid (hp : p.valid) : (@decorate_error α msg p).valid :=
+decorate_errors.valid hp
+
+@[simp] lemma any_char.valid : valid any_char :=
+begin
+  intros cb n,
+  simp only [any_char],
+  split_ifs,
+  { simpa only [true_and, zero_le, le_add_iff_nonneg_right,
+                parse_result.pos] using nat.le_of_succ_le},
+  { simp only [imp_self, and_true, parse_result.pos] }
+end
+
+@[simp] lemma sat.valid {p : char → Prop} [decidable_pred p] : valid (sat p) :=
+begin
+  intros cb n,
+  simp only [sat],
+  split_ifs,
+  { simpa only [true_and, zero_le, le_add_iff_nonneg_right,
+                parse_result.pos] using nat.le_of_succ_le },
+  { simp only [imp_self, and_true, parse_result.pos] },
+  { simp only [parse_result.pos, imp_self, and_true] }
+end
+
+@[simp] lemma eps.valid : valid eps := pure.valid
+
+lemma ch.valid {c : char} : valid (ch c) := decorate_error.valid (sat.valid.and_then eps.valid)
+
+lemma char_buf.valid {s : char_buffer} : valid (char_buf s) :=
+decorate_error.valid (valid.mmap' (λ _ _, ch.valid))
+
+end valid_parsers
+
+end defn_lemmas
+
+end parser
